examples/scheduler/include/fdsched/message.h
@@ -23,7 +23,8 @@ struct [[rc::parameters("cont : type")]]
   struct message *next;
 
 #define MAX_MESSAGE_LEN (4096 - sizeof(message_type_t) - sizeof(size_t) - sizeof(struct message*))
-  [[rc::field("array<u8, {get_packet_data (m_id data) `at_type` int u8}>")]]
+  [[rc::field("array_p<u8,{(get_packet_data data.(m_id)) `at_type` int u8},"
+	      "{Z.to_nat max_msg_len}>")]]
   uint8_t data[MAX_MESSAGE_LEN];
 };
 
@@ -31,16 +32,18 @@ struct [[rc::parameters("cont : type")]]
    function */
 [[rc::parameters("msg : message_data", "q : loc")]]
 [[rc::args("q @ &own<struct<struct_message,"
-     "uninit<u8>,"
-	   "{m_length msg} @ int<u64>,"
-	   "uninit<void*>,"
-	   "array<u8, {get_packet_data (m_id msg) `at_type` int u8}>>>")]]
-[[rc::returns("{message_identify_type_coq (m_id msg)} @ int<u8>")]]
-[[rc::ensures("own q : struct<struct_message,"
 	   "uninit<u8>,"
 	   "{m_length msg} @ int<u64>,"
 	   "uninit<void*>,"
-	   "array<u8, {get_packet_data (m_id msg) `at_type` int u8}>>")]]
+	   "array_p<u8, {(get_packet_data  msg.(m_id)) `at_type` int u8},"
+	   "{Z.to_nat max_msg_len}>>>")]]
+[[rc::returns("{message_identify_type_coq msg.(m_id)} @ int<u8>")]]
+[[rc::ensures("own q : struct<struct_message,"
+	      "uninit<u8>,"
+	      "{m_length msg} @ int<u64>,"
+	      "uninit<void*>,"
+	      "array_p<u8,{get_packet_data msg.(m_id) `at_type` int(u8)},"
+	      "{Z.to_nat max_msg_len}>>")]]
 message_type_t message_identify_type(struct message* msg);
 
 
@@ -48,7 +51,7 @@ message_type_t message_identify_type(struct message* msg);
 struct [[rc::refined_by("messages : {list message_data}")]]
        [[rc::typedef("message_queue : ∃ p. own_constrained<tyown_constraint<p, null>, ...>")]]
     message_queue {
-  [[rc::field("tyfold<{(λ data cont, &own (data @ message cont) : type) <$> messages}, place<p>>")]]
+  [[rc::field("tyfold<{(λ data cont, &own (malloced (ly_size struct_message) (data @ message cont)) : type) <$> messages}, place<p>>")]]
   struct message *first;
   [[rc::field("&own<place<p>>")]]
   struct message **last;
@@ -57,7 +60,7 @@ struct [[rc::refined_by("messages : {list message_data}")]]
 /* enqueue at end */
 [[rc::parameters("data : {list message_data}", "msg : message_data", "q : loc")]]
 [[rc::args("q @ &own<data @ message_queue>",
-           "&own<msg @ message<uninit<void*>>>")]]
+           "&own<malloced<{ly_size struct_message}, msg @ message<uninit<void*>>>>")]]
 [[rc::ensures("own q : {data ++ [msg]} @ message_queue")]]
 static inline
 void message_queue_add(struct message_queue *q, struct message *msg) {
@@ -81,7 +84,7 @@ int message_queue_empty(struct message_queue *q) {
 [[rc::parameters("data : {list message_data}", "q : loc")]]
 [[rc::args("q @ &own<data @ message_queue>")]]
 [[rc::requires("{data ≠ []}")]]
-[[rc::returns("{head data} @ optionalO<λ msg1. &own<msg1 @ message<uninit<void*>>>>")]]
+[[rc::returns("{head data} @ optionalO<λ msg1. &own<malloced<{ly_size struct_message}, msg1 @ message<uninit<void*>>>>>")]]
 [[rc::ensures("own q : {tail data} @ message_queue")]]
 static inline
 struct message* message_queue_remove(struct message_queue *q) {
