examples/scheduler/src/proofs/fdsched/fdsched_extra.v
@@ -9,10 +9,10 @@ Record fd_sched := {
     sched_state : npfp_sched;
   }.
 
-(**TODO: upstream*)
+(* TODO: upstream *)
 Notation array_p ly elts n :=
-  (array ly (elts ++ replicate n (uninit ly)))
-    (only parsing). 
+  (array ly (elts ++ replicate (n - length elts) (uninit ly)))
+  (only parsing).
 
 Program Definition fds_set_callback_func (fds : fd_sched)  (type prio : nat) :=
   {|
@@ -36,3 +36,169 @@ Definition fds_add_channel_func (fd_state : fd_sched) (fd : FD) :=
     sched_state := fd_state.(sched_state)
   |}.
 
+Section RecieveOneMessageSpecification.
+
+  Context `{!PacketArrivals}.
+
+   (** Given a packet ID, generate the message corresponding to that packet ID *)
+  Definition generate_msg_corresponding_to_packetID (id : packet_ID) : message_data :=
+    {|m_type := inhabitant; m_length := max_msg_len; m_id := id|}.
+
+  (** if pending packets is empty then add nothing to the scheduler else add
+      the right message to the scheduler. *)
+  Definition add_pending_msg_to_scheduler (t :nat) (l1 : list LogEntry) (fd : FD) (sched_state : npfp_sched) : npfp_sched :=
+    let ID := (get_head_ID t l1 fd) in
+    let pending := get_pending_packets_from_given_fd t l1 fd in
+    if decide (pending = []) then sched_state else
+      let msg := generate_msg_corresponding_to_packetID ID in
+      npfp_enqueue_func sched_state msg.
+
+  Definition receive_one_message_func (t :nat) (l : list LogEntry) (fd :FD) (fd_state : fd_sched) : fd_sched :=
+    {|
+      input_channels := fd_state.(input_channels);
+      sched_state := add_pending_msg_to_scheduler t l fd fd_state.(sched_state);
+    |}.
+
+End RecieveOneMessageSpecification.
+
+Section RecieveOneMessageProof.
+  Context `{!PacketArrivals} `{!typeG Σ}.
+
+  Global Instance simpl_and_npfp_enqueue_func fd_state msg1 msg2:
+    SimplAndUnsafe (npfp_enqueue_func (sched_state fd_state) msg1 =
+                    npfp_enqueue_func (sched_state fd_state) msg2) (msg1 = msg2) .
+  Proof. by move => ->. Qed.
+
+  Global Instance simpl_and_get_packet_data_option_inst (n : packet_ID) t1 l fd
+    `{CanSolve (is_Some (get_head_ID_option t1 l fd))}
+    `{!IsEx n}:
+    SimplAndUnsafe
+      (get_packet_data_option (get_head_ID_option t1 l fd) `at_type` (int u8) ++
+         replicate (Z.to_nat max_msg_len -
+                      length (get_packet_data_option (get_head_ID_option t1 l fd)))
+         (uninit u8) =
+         get_packet_data  n `at_type` (int u8) ++
+           replicate (Z.to_nat max_msg_len - length (get_packet_data_option (Some n)))
+           (uninit u8))%I
+      (n = hd inhabitant (get_pending_packets_from_given_fd t1 l fd)).
+  Proof.
+    rename select (CanSolve _) into HSome.
+    rewrite /CanSolve /get_head_ID_option in HSome.
+    move => ->.
+    case (get_pending_packets_from_given_fd t1 l fd) eqn: EQ; first by contradict HSome.
+    by rewrite /get_head_ID_option EQ //=.
+  Qed.
+
+  Global Instance simpl_and_message_equality msg1 msg2 :
+    SimplAnd (msg1 = msg2)
+      (msg1.(m_type) = msg2.(m_type)
+       ∧ msg1.(m_length) = msg2.(m_length)
+       ∧ msg1.(m_id) = msg2.(m_id)).
+  Proof. destruct msg1, msg2. split; naive_solver. Qed.
+
+  Lemma recvonemsg0 t1 l fd:
+    (if bool_decide (is_Some (get_head_ID_option t1 l fd)) then max_msg_len else -1) ≤ 0 →
+    ∃ n' : nat,
+      (get_packet_data_option (get_head_ID_option t1 l fd) `at_type` (int u8))%I =
+        replicate n' (uninit u8)
+      ∧ replicate (Z.to_nat max_msg_len - length (get_packet_data_option (get_head_ID_option t1 l fd)))
+          (uninit u8) =
+          replicate
+            (length (get_packet_data_option (get_head_ID_option t1 l fd)) +
+               (Z.to_nat max_msg_len - length (get_packet_data_option (get_head_ID_option t1 l fd))) - n')
+            (uninit u8)
+      ∧ (n' <=
+           length (get_packet_data_option (get_head_ID_option t1 l fd)) +
+             (Z.to_nat max_msg_len - length (get_packet_data_option (get_head_ID_option t1 l fd))))%nat.
+  Proof.
+    exists 0%nat; split.
+    * unfold_opaque @get_packet_data_option.
+      have Hfalse: (¬ is_Some (get_head_ID_option t1 l fd)) by solve_goal.
+      rewrite -eq_None_not_Some in Hfalse.
+      by rewrite Hfalse.
+    * split; try solve_goal.
+      have Hfalse: (¬ is_Some (get_head_ID_option t1 l fd)) by solve_goal.
+      rewrite -eq_None_not_Some in Hfalse.
+      rewrite Hfalse. unfold_opaque @get_packet_data_option.
+      simpl.
+      solve_goal.
+  Qed.
+
+  Lemma recvonemsg1 t1 l fd:
+     (if bool_decide (is_Some (get_head_ID_option t1 l fd)) then max_msg_len else -1) ≤ 0 →
+     (ly_size u8 * 4079)%nat =
+  (ly_size u8 *
+   (length (get_packet_data_option (get_head_ID_option t1 l fd)) +
+      (Z.to_nat max_msg_len - length (get_packet_data_option (get_head_ID_option t1 l fd)))))%nat.
+  Proof.
+    move => ?.
+    have Hfalse: (¬ is_Some (get_head_ID_option t1 l fd)) by solve_goal.
+    rewrite -eq_None_not_Some in Hfalse.
+    rewrite !Hfalse. unfold_opaque @get_packet_data_option.
+    simpl.
+    solve_goal.
+    Qed.
+
+  Lemma recvonemsg2 t1 l fd :
+    (if bool_decide (is_Some (get_head_ID_option t1 l fd)) then max_msg_len else -1) ≤ 0 →
+    (if bool_decide (is_Some (get_head_ID_option t1 l fd)) then max_msg_len else -1) =
+      (if decide (get_pending_packets_from_given_fd t1 l fd = []) then -1 else 0).
+  Proof.
+    move => ?.
+    rewrite /get_head_ID_option.
+    case (get_pending_packets_from_given_fd t1 l fd) eqn:EQ; first by done.
+    have Hfalse: bool_decide (is_Some (get_head_ID_option t1 l fd)) = false by solve_goal.
+    by rewrite /get_head_ID bool_decide_eq_false -eq_None_not_Some head_None EQ in Hfalse.
+  Qed.
+
+  Lemma recvonemsg3 t1 l fd fd_state :
+    (if bool_decide (is_Some (get_head_ID_option t1 l fd)) then max_msg_len else -1) ≤ 0 →
+    fd_state = receive_one_message_func t1 l fd fd_state.
+  Proof.
+    move => ?.
+    have Hfalse: bool_decide (is_Some (get_head_ID_option t1 l fd)) = false by solve_goal.
+    rewrite /get_head_ID bool_decide_eq_false -eq_None_not_Some head_None in Hfalse.
+    rewrite /receive_one_message_func /add_pending_msg_to_scheduler !Hfalse //=.
+    destruct fd_state; f_equiv; done.
+  Qed.
+
+  Lemma recvonemsg4 t1 l fd :
+    ¬ (if bool_decide (is_Some (get_head_ID_option t1 l fd)) then max_msg_len else -1) ≤ 0 →
+    0 = (if decide (get_pending_packets_from_given_fd t1 l fd = []) then -1 else 0).
+  Proof.
+    move => ?.
+    have Htrue: bool_decide (is_Some (get_head_ID_option t1 l fd)) = true by solve_goal.
+    rewrite /get_head_ID_option bool_decide_eq_true in Htrue.
+    rewrite decide_bool_decide.
+    case (bool_decide (get_pending_packets_from_given_fd t1 l fd = [])) eqn: EQ; try done.
+    rewrite bool_decide_eq_true in EQ.
+    rewrite EQ in Htrue.
+    by contradict Htrue.
+  Qed.
+
+  Lemma recvonemsg5 t1 l fd fd_state:
+    ¬ (if bool_decide (is_Some (get_head_ID_option t1 l fd)) then max_msg_len else -1) ≤ 0 →
+    npfp_enqueue_func (sched_state fd_state)
+                      {|
+                        m_type :=
+                          message_identify_type_coq
+                            (hd inhabitant (get_pending_packets_from_given_fd t1 l fd));
+                        m_length := if bool_decide (is_Some (get_head_ID_option t1 l fd))
+                                    then max_msg_len else -1;
+                        m_id := hd inhabitant (get_pending_packets_from_given_fd t1 l fd)
+                      |}
+    = add_pending_msg_to_scheduler t1 l fd (sched_state fd_state).
+  Proof.
+    move => ?.
+    have Htrue: bool_decide (is_Some (get_head_ID_option t1 l fd)) = true by solve_goal.
+    rewrite  /add_pending_msg_to_scheduler !Htrue //= decide_bool_decide.
+    rewrite bool_decide_eq_true /get_head_ID_option in Htrue.
+    have ->: bool_decide (get_pending_packets_from_given_fd t1 l fd = []) = false
+        by rewrite bool_decide_eq_false -head_is_Some.
+    rewrite /get_priority /npfp_enqueue_func.
+    case (get_pending_packets_from_given_fd t1 l fd) eqn:EQ; first by contradict Htrue.
+    f_equiv; rewrite /hd; last by rewrite /get_head_ID /get_head_ID_option EQ //=.
+    by rewrite /generate_msg_corresponding_to_packetID /get_head_ID /get_head_ID_option EQ //= max_msg_len_simpl.
+  Qed.
+
+End RecieveOneMessageProof.
