examples/scheduler/src/proofs/fdsched/message_extra.v
@@ -1,9 +1,6 @@
 From refinedc.typing Require Import typing.
 From refinedc.examples.scheduler.src.fdsched Require Export basic_definitions.
 
-Definition max_msg_len : Z :=
-  4096 - ly_size u8 - ly_size size_t - ly_size void*.
-
 #[projections(primitive)]
 Record message_data := Message {
   m_type : nat;
@@ -11,13 +8,8 @@ Record message_data := Message {
   m_id : packet_ID
 }.
 
-Global Instance packet_ID_inhabited : Inhabited packet_ID :=
-  populate (PACKET_ID inhabitant inhabitant inhabitant).
-
 Global Instance message_data_inhabited : Inhabited message_data :=
   populate (Message inhabitant inhabitant inhabitant).
-
-Notation num_msg_types := (max_int u8 + 1) (only parsing).
 
 (** function to set type of a message to a given value*)
 Definition set_msg_type (msg : message_data) (type : nat) := {|
@@ -25,11 +17,6 @@ Definition set_msg_type (msg : message_data) (type : nat) := {|
   m_length := m_length msg;
   m_id := m_id msg
 |}.
-
-(** function to look up the type of the message *)
-Axiom message_identify_type_coq : packet_ID → nat.
-
-Axiom msg_type_bounded: ∀ msg : message_data, message_identify_type_coq (m_id msg) < num_msg_types.
 
 (** sets the type field of the message to the correct type *)
 Definition update_msg_type (msg : message_data) : message_data :=
