examples/scheduler/src/proofs/fdsched/axioms.v
@@ -1,0 +1,32 @@
+From refinedc.typing Require Export typing.
+
+(** Wrapper type for file descriptors *)
+Notation FD := Z (only parsing).
+
+(** the ID for a packet is given by a tuple of fd, time and index in the arrivals at that time *)
+Record packet_ID := PACKET_ID {
+  fd : FD;
+  arr_time : nat;
+  index : nat;
+}.
+
+(** The data type for interesting events we record in the log*)
+Inductive LogEntry :=
+| read_from_socket (j : packet_ID) (t : nat)
+| callback_dispatched (j : packet_ID) (t : nat)
+| callback_returned (j : packet_ID) (t : nat).
+
+Section EventLog.
+  Context `{typeG Σ}.
+
+  Axiom curr_time : nat → iProp Σ.
+  Axiom curr_log : list LogEntry → iProp Σ.
+
+End EventLog.
+
+(** function to look up the type of the message *)
+Notation num_msg_types := (max_int u8 + 1) (only parsing).
+
+Axiom message_identify_type_coq : packet_ID → nat.
+
+Axiom msg_type_bounded : ∀ msg, message_identify_type_coq msg < num_msg_types.
